coq/Casts.v
@@ -1,6 +1,9 @@
 Require Import ssreflect. 
 Require Import Eqdep.
-Require Import JMeq.
+Require Import JMeq Program.Equality.
+Set Implicit Arguments.
+Unset Strict Implicit.
+Import Prenex Implicits.
 
 (*===========================================================================
     Casts, borrowed from Adam Chlipala's Lambda Tamer library
@@ -9,8 +12,11 @@ Notation "e :? pf" := (eq_rect _ (fun X : _ => X) e _ pf)
   (no associativity, at level 90).
 
 Lemma cast_id A (x:A) (pf:A=A) : (x :? pf) = x.
-Proof. unfold eq_rect. by rewrite (UIP_refl _ A pf). Qed.
+Proof. by rewrite /eq_rect (UIP_refl _ A pf). Qed.
 
+Lemma cast_UIP A B (a:A) (pf1:A=B) (pf2:A=B) :
+  (a :? pf1) = (a :? pf2).
+Proof. by rewrite (UIP _ A B pf1 pf2). Qed.
 
 Theorem cast_coalesce T1 T2 T3 (e : T1) (pf1 : T1 = T2) (pf2 : T2 = T3):
   ((e :? pf1) :? pf2) = (e :? trans_eq pf1 pf2).
@@ -27,16 +33,16 @@ Lemma trans_cast T1 T2 H (x z : T1) (y : T2):
   x = (y :? H)
   -> (y :? H) = z
   -> x = z.
-Proof.  move <- => ->. done. Qed.
+Proof. by move <- => ->. Qed.
 
 Lemma cast_JMeq A B (x: A) (H: A=B): JMeq x (x :? H).
 Proof. unfold eq_rect. by case H. Qed.
 
 Lemma cast_sym A B (pf: A=B) x: ((x :? sym_equal pf) :? pf) = x.
-Proof. have H := cast_coalesce B A B x (sym_equal pf) pf. by subst. Qed.
+Proof. have H := cast_coalesce x (sym_equal pf) pf. by subst. Qed.
 
 Lemma cast_sym_opp A B (pf: A=B) x: ((x :? pf) :? sym_equal pf) = x.
-Proof. have H := cast_coalesce A B A x pf (sym_equal pf). by subst. Qed. 
+Proof. have H := cast_coalesce x pf (sym_equal pf). by subst. Qed. 
 
 Definition prod_eq A B A' B' (pfA: A=A') (pfB: B=B'): (A*B = A'*B')%type.
 Proof. congruence. Defined. 
@@ -47,56 +53,65 @@ Proof. congruence. Defined.
 Definition arrow_eq A B A' B' (pfA: A=A') (pfB: B=B'): ((A->B) = (A'->B'))%type.
 Proof. congruence. Defined. 
 
-Implicit Arguments prod_eq [A B A' B'].
-Implicit Arguments sum_eq [A B A' B'].
-Implicit Arguments arrow_eq [A B A' B'].
-
-Require Import Program.Equality.
-
-Lemma cast_fst :
-  forall (A B A' B':Type),
-  forall (pfA:A=A') (pfB:B=B') (p:A*B),
+Lemma cast_fstAux A B A' B' (pfA:A=A') (pfB:B=B') (p:A*B):
   fst (p :? prod_eq pfA pfB) = (fst p :? pfA).
-Proof. intros. unfold eq_rect. case pfA. unfold prod_eq, trans_eq, f_equal. case pfB. trivial.
-Qed.
+Proof. rewrite/eq_rect. case pfA. rewrite/prod_eq/trans_eq/f_equal. by case pfB. Qed.
 
-Lemma cast_snd :
-  forall (A B A' B':Type),
-  forall (pfA:A=A') (pfB:B=B') (p:A*B),
+Lemma cast_sndAux A B A' B' (pfA:A=A') (pfB:B=B') (p:A*B):
   snd (p :? prod_eq pfA pfB) = (snd p :? pfB).
-intros. unfold eq_rect. case pfA. unfold prod_eq, trans_eq, f_equal. case pfB. trivial.
-Qed.
+Proof. rewrite /eq_rect. case pfA. rewrite/prod_eq/trans_eq/f_equal. by case pfB. Qed.
 
-Lemma cast_inl :
-  forall (A B A' B':Type),
-  forall (pfA:A=A') (pfB:B=B') (a:A),
+Lemma cast_pairAux A B A' B' (pfA:A=A') (pfB:B=B') (x:A) (y:B):
+  ((x,y) :? prod_eq pfA pfB) = (x :? pfA, y :? pfB).
+Proof. rewrite /eq_rect. case pfA. rewrite/prod_eq/trans_eq/f_equal. by case pfB. Qed.
+
+Lemma cast_fst A B A' B' (pfA:A=A') (pfB:B=B') (pfAB: (A*B)%type=(A'*B')%type) (p:A*B):
+  fst (p :? pfAB) = (fst p :? pfA).
+Proof. rewrite -(cast_UIP _ (prod_eq pfA pfB)). apply cast_fstAux. Qed.
+
+Lemma cast_snd A B A' B' (pfA:A=A') (pfB:B=B') (pfAB: (A*B)%type=(A'*B')%type) (p:A*B):
+  snd (p :? pfAB) = (snd p :? pfB).
+Proof. rewrite -(cast_UIP _ (prod_eq pfA pfB)). apply cast_sndAux. Qed.
+
+Lemma cast_pair A B A' B' (pfA:A=A') (pfB:B=B') (pfAB: (A*B)%type=(A'*B')%type) (x:A) (y:B):
+  ((x,y) :? pfAB) = (x :? pfA, y :? pfB).
+Proof. rewrite -(cast_UIP _ (prod_eq pfA pfB)). apply cast_pairAux. Qed.
+
+Lemma cast_inlAux A B A' B' (pfA:A=A') (pfB:B=B') (a:A):
   (inl _ a :? sum_eq pfA pfB) = (inl _ (a :? pfA)).
-intros. unfold eq_rect. case pfA. unfold sum_eq, trans_eq, f_equal. case pfB. trivial.
-Qed.
+Proof. rewrite /eq_rect. case pfA. unfold sum_eq, trans_eq, f_equal. by case pfB. Qed.
 
-Lemma cast_inr :
-  forall (A B A' B':Type),
-  forall (pfA:A=A') (pfB:B=B') (b:B),
+Lemma cast_inrAux A B A' B' (pfA:A=A') (pfB:B=B') (b:B):
   (inr _ b :? sum_eq pfA pfB) = (inr _ (b :? pfB)).
-intros. unfold eq_rect. case pfA. unfold sum_eq, trans_eq, f_equal. case pfB. trivial.
-Qed.
+Proof. rewrite /eq_rect. case pfA. unfold sum_eq, trans_eq, f_equal. by case pfB. Qed.
 
-Lemma cast_app :
+Lemma cast_inl A B A' B' (pfA: A=A') (pfB: B=B') (pfAB: (A+B)%type = (A'+B')%type) (a:A) :
+  (inl _ a :? pfAB) = (inl _ (a :? pfA)).
+Proof. rewrite -(cast_UIP _ (sum_eq pfA pfB)). apply cast_inlAux. Qed. 
+
+Lemma cast_inr A B A' B' (pfA: A=A') (pfB: B=B') (pfAB: (A+B)%type = (A'+B')%type) (b:B) :
+  (inr _ b :? pfAB) = (inr _ (b :? pfB)).
+Proof. rewrite -(cast_UIP _ (sum_eq pfA pfB)). apply cast_inrAux. Qed. 
+
+Lemma cast_appAux :
   forall (A B A' B':Type),
   forall (pfA:A=A') (pfB:B=B') (f:A->B) (a:A),
   ((f a) :? pfB) = (f :? arrow_eq pfA pfB) (a :? pfA).
-intros. unfold eq_rect. case pfA. case pfB. unfold arrow_eq, trans_eq, f_equal. trivial.
+intros. unfold eq_rect, f_equal. case pfA. case pfB. unfold arrow_eq, trans_eq, f_equal. trivial.
 Qed.
 
-Implicit Arguments cast_fst [A B A' B'].
-Implicit Arguments cast_snd [A B A' B'].
-Implicit Arguments cast_inl [A B A' B'].
-Implicit Arguments cast_inr [A B A' B'].
-Implicit Arguments cast_app [A B A' B'].
+Lemma cast_app A B A' B' (pfA:A=A') (pfB:B=B') (pfAB: (A->B)=(A'->B')) (f:A->B) (a:A):
+  ((f a) :? pfB) = (f :? pfAB) (a :? pfA).
+Proof. rewrite -(cast_UIP _ (arrow_eq pfA pfB)). apply cast_appAux. Qed.
 
-
-Lemma cast_UIP : forall (A B:Type) (a:A) (pf1:A=B) (pf2:A=B),
-  (a :? pf1) = (a :? pf2).
-intros. 
-rewrite (UIP _ A B pf1 pf2). trivial.
+Lemma cast_appFunAux :
+  forall (A B A' B':Type),
+  forall (pfA:A=A') (pfB:B=B') (f:A->B) (a:A'),
+  (f :? arrow_eq pfA pfB) a = (f (a:?sym_equal pfA) :? pfB).
+intros. unfold eq_rect, f_equal. case pfB. unfold arrow_eq, trans_eq, f_equal. by destruct pfA. 
 Qed.
+
+
+Lemma cast_appFun A A' B B' (pfA:A=A') (pfB:B=B') (pfAB: (A->B)=(A'->B')) (f:A->B) (a:A'):
+  (f :? pfAB) a = (f (a :? sym_equal pfA) :? pfB).
+Proof. rewrite -(cast_UIP _ (arrow_eq pfA pfB)). by rewrite -cast_appFunAux.  Qed.
